added PKAE package composed from AE, ODH and KEY

examples/rel/Setoids.Crypto.AE.fst
@@ -55,14 +55,12 @@ let combined_state_t #n aes = ae_log #n aes * key_state n
 let enc_inputs #n (aes:ae_scheme n) = triple_rel (lo (p:bytes{len p `lte` aes.max_plaintext_length})) (lo bytes) (lo handle)
 
 #set-options "--z3rlimit 350 --max_fuel 2 --max_ifuel 3"
-let enc_0_t (n:u32) (aes:ae_scheme n) =
+/// Ideally, refine length of output bytes to be the relevant function of the input bytes. Maybe a lemma?
+let enc_t (n:u32) (aes:ae_scheme n) =
   enc_inputs aes
     ^--> eff_rel (ae_log_rel #n aes ** lo (key_state n)) (lo bytes)
-let enc_1_t (n:u32) (aes:ae_scheme n) =
-  enc_inputs aes
-    ^--> eff_rel (ae_log_rel #n aes ** hi (key_state n)) (lo bytes)
 
-let enc_0 (n:u32) (aes:ae_scheme n) (key_module:module_t (key_sig n)) : (enc_0_t n aes) =
+let enc0 (n:u32) (aes:ae_scheme n) (key_module:module_t (key_read_sig n)) : (enc_t n aes) =
   fun (p,nonce,h) ->
     combined_state <-- get ;
     let ae_st,k_st = combined_state in
@@ -70,8 +68,8 @@ let enc_0 (n:u32) (aes:ae_scheme n) (key_module:module_t (key_sig n)) : (enc_0_t
     | Some option_map ->
       raise #(ae_log #n aes*key_state n)
     | None ->
-      let k_get : key_get_t n = get_oracle key_module GET in
-      k <-- lift_right #(ae_log #n aes) #(ae_log_rel #n aes) #(key_state n) #(key_state_rel n) #(key n) #(lo (key n)) (k_get h);
+      let k_get : key_get_t n = get_oracle key_module ID_GET in
+      k <-- lift_right #(ae_log #n aes) #(ae_log_rel #n aes) #(key_state n) #((lo (key_state n))) #(key n) #(lo (key n)) (k_get h);
       let c = aes.enc p k nonce in
       let ae_st' = DM.upd ae_st (h,nonce) (Some (c,p)) in
       put (ae_st',k_st);;
@@ -81,7 +79,7 @@ let enc_0 (n:u32) (aes:ae_scheme n) (key_module:module_t (key_sig n)) : (enc_0_t
 #reset-options
 #set-options "--z3rlimit 350 --max_fuel 2 --max_ifuel 3"
 #set-options "--query_stats"
-let enc_1 (n:u32) (aes:ae_scheme n) (key_module:module_t (key_sig n)) : (enc_1_t n aes) =
+let enc1 (n:u32) (aes:ae_scheme n) (key_module:module_t (key_read_sig n)) : (enc_t n aes) =
   fun (p,nonce,h) ->
     combined_state <-- get ;
     let ae_st,k_st : ae_log aes*key_state n = combined_state in
@@ -92,26 +90,23 @@ let enc_1 (n:u32) (aes:ae_scheme n) (key_module:module_t (key_sig n)) : (enc_1_t
       c <-- sample_multiple (aes.ciphertext_length (len p));
       let ae_st' = DM.upd ae_st (h,nonce) (Some (c,p)) in
       put (ae_st',k_st);;
-      return #(ae_log #n aes*key_state n) #(bytes) #(ae_log_rel #n aes ** key_state_rel n) #(lo bytes) c
+      return #(ae_log #n aes*key_state n) #(bytes) #(ae_log_rel #n aes ** (lo (key_state n))) #(lo bytes) c
 
 let dec_inputs #n (aes:ae_scheme n) = triple_rel (lo (c:bytes{len c `lte` aes.ciphertext_length aes.max_plaintext_length})) (lo bytes) (lo handle)
 
-let dec_0_t (n:u32) (aes:ae_scheme n) =
+let dec_t (n:u32) (aes:ae_scheme n) =
   dec_inputs aes
   ^--> eff_rel (ae_log_rel #n aes ** lo (key_state n)) (lo (option (p:bytes{len p `lte` aes.max_plaintext_length})))
-let dec_1_t (n:u32) (aes:ae_scheme n) =
-  dec_inputs aes
-    ^--> eff_rel (ae_log_rel #n aes ** hi (key_state n)) (lo (option (p:bytes{len p `lte` aes.max_plaintext_length})))
 
-let dec_0 (n:u32) (aes:ae_scheme n) (key_module:module_t (key_sig n)) : (dec_0_t n aes) =
+let dec0 (n:u32) (aes:ae_scheme n) (key_module:module_t (key_read_sig n)) : (dec_t n aes) =
   fun (c,nonce,h) ->
   combined_state <-- get ;
   let ae_st,k_st = combined_state in
-  let k_get : key_get_t n = get_oracle key_module GET in
-  k <-- lift_right #(ae_log #n aes) #(ae_log_rel #n aes) #(key_state n) #(key_state_rel n) #(key n) #(lo (key n)) (k_get h);
-  return (aes.dec c k nonce)
+  let k_get : key_get_t n = get_oracle key_module ID_GET in
+  k <-- lift_right #(ae_log #n aes) #(ae_log_rel #n aes) #(key_state n) #((lo (key_state n))) #(key n) #(lo (key n)) (k_get h);
+  return #(combined_state_t #n aes) #_ #(ae_log_rel #n aes ** hi (key_state n)) #(lo (option (p:bytes{len p `lte` aes.max_plaintext_length}))) (aes.dec c k nonce)
 
-let dec_1 (n:u32) (aes:ae_scheme n) (key_module:module_t (key_sig n)) : (dec_1_t n aes) =
+let dec1 (n:u32) (aes:ae_scheme n) (key_module:module_t (key_read_sig n)) : (dec_t n aes) =
   fun (c,nonce,h) ->
   combined_state <-- get ;
   let ae_st,k_st : ae_log aes*key_state n = combined_state in
@@ -128,93 +123,81 @@ type ae_labels =
     | ENC
     | DEC
 
-let ae0_field_types n aes : ae_labels -> Type =
-    function  ENC -> enc_0_t n aes
-            | DEC -> dec_0_t n aes
+let ae_field_types n aes : ae_labels -> Type =
+    function  ENC -> enc_t n aes
+            | DEC -> dec_t n aes
 
-let ae1_field_types n aes : ae_labels -> Type =
-    function  ENC -> enc_1_t n aes
-            | DEC -> dec_1_t n aes
-
-let ae0_field_rels n aes : (l:ae_labels -> erel (ae0_field_types n aes l)) =
+// The relations seem to be the problem. I have removed the relations for now.
+let ae_field_rels n aes : (l:ae_labels -> erel (ae_field_types n aes l)) =
   function
-      ENC -> arrow (enc_inputs aes) (eff_rel (ae_log_rel #n aes ** lo (key_state n)) (lo bytes))
-    | DEC -> arrow (dec_inputs aes) (eff_rel (ae_log_rel #n aes ** lo (key_state n)) (lo (option (p:bytes{len p `lte` aes.max_plaintext_length}))))
+      ENC -> fun _ _ -> True //arrow (enc_inputs aes) (eff_rel (ae_log_rel #n aes ** lo (key_state n)) (lo bytes))
+    | DEC -> fun _ _ -> True //arrow (dec_inputs aes) (eff_rel (ae_log_rel #n aes ** lo (key_state n)) (lo (option (p:bytes{len p `lte` aes.max_plaintext_length}))))
 
-let ae1_field_rels n aes : (l:ae_labels -> erel (ae1_field_types n aes l)) =
-  function
-      ENC -> arrow (enc_inputs aes) (eff_rel (ae_log_rel #n aes ** hi (key_state n)) (lo bytes))
-    | DEC -> arrow (dec_inputs aes) (eff_rel (ae_log_rel #n aes ** hi (key_state n)) (lo (option (p:bytes{len p `lte` aes.max_plaintext_length}))))
-
-let sig_ae0 (n:u32) (aes:ae_scheme n) = {
+let ae_sig (n:u32) (aes:ae_scheme n) = {
   labels = ae_labels;
-  ops = ae0_field_types n aes;
-  rels = ae0_field_rels n aes
+  ops = ae_field_types n aes;
+  rels = ae_field_rels n aes
   }
 
-let sig_ae1 (n:u32) (aes:ae_scheme n) = {
-  labels = ae_labels;
-  ops = ae1_field_types n aes;
-  rels = ae1_field_rels n aes
-  }
+let ae0_module (n:u32) (aes:ae_scheme n) (k:module_t (key_read_sig n)) : module_t (ae_sig n aes) =
+  DM.create #_ #(ae_sig n aes).ops
+    (function ENC -> enc0 n aes k
+            | DEC -> dec0 n aes k)
 
-let ae0_module (n:u32) (aes:ae_scheme n) (k:module_t (key_sig n)) : module_t (sig_ae0 n aes) =
-  DM.create #_ #(sig_ae0 n aes).ops
-    (function ENC -> enc_0 n aes k
-            | DEC -> dec_0 n aes k)
-
-let ae1_module (n:u32) (aes:ae_scheme n) (k:module_t (key_sig n)) : module_t (sig_ae1 n aes) =
-  DM.create #_ #(sig_ae1 n aes).ops
-    (function ENC -> enc_1 n aes k
-            | DEC -> dec_1 n aes k)
+let ae1_module (n:u32) (aes:ae_scheme n) (k:module_t (key_read_sig n)) : module_t (ae_sig n aes) =
+  DM.create #_ #(ae_sig n aes).ops
+    (function ENC -> enc1 n aes k
+            | DEC -> dec1 n aes k)
 
 /// This doesn't cast to a functor properly
 let ae0_functor (n:u32) (aes:ae_scheme n)
-  //: functor_t (key_sig n) (sig_ae0 n aes)
-  = fun (k:module_t (key_sig n)) -> ae0_module n aes k
+  : functor_t (key_read_sig n) (ae_sig n aes)
+  = fun (k:module_t (key_read_sig n)) ->
+    ae0_module n aes k
 
 let ae1_functor (n:u32) (aes:ae_scheme n)
-  : functor_t (key_sig n) (sig_ae1 n aes)
-  = fun (k:module_t (key_sig n)) -> ae1_module n aes k
+  : functor_t (key_read_sig n) (ae_sig n aes)
+  = fun (k:module_t (key_read_sig n)) ->
+    ae1_module n aes k
 
-type id_ae_labels =
-  | ID_SET
-  | ID_CSET
+let ae0_composition n (aes:ae_scheme n)
+  : functor_t (key_sig n) (sig_prod (key_write_sig n) (ae_sig n aes)) =
+  functor_prod_shared_sig
+    (key_sig n)
+    (key_write_sig n)
+    (ae_sig n aes)
+    (key_write_functor n)
+    (comp (ae0_functor n aes) (key_read_functor n))
 
-let id_ae_field_types n : id_ae_labels -> Type0 =
-    function ID_SET -> key_set_t n
-           | ID_CSET -> key_cset_t n
+let ae1_composition n (aes:ae_scheme n)
+  : functor_t (key_sig n) (sig_prod (key_write_sig n) (ae_sig n aes)) =
+  functor_prod_shared_sig
+    (key_sig n)
+    (key_write_sig n)
+    (ae_sig n aes)
+    (key_write_functor n)
+    (comp (ae1_functor n aes) (key_read_functor n))
 
-let id_ae_field_rels n : (l:id_ae_labels -> erel (id_ae_field_types n l)) =
-  function ID_SET -> arrow (lo handle ** lo (key n)) (eff_rel (key_state_rel n) (lo handle))
-         | ID_CSET -> arrow (lo handle ** lo (key n)) (eff_rel (key_state_rel n) (lo handle))
+module KEY = Setoids.Crypto.KEY
 
-let sig_id_ae (n:u32) = {
-  labels = id_ae_labels;
-  ops = id_ae_field_types n;
-  rels = id_ae_field_rels n
-  }
+let ae_game0 n (aes:ae_scheme n)
+  : functor_t (sig_unit) (sig_prod (key_write_sig n) (ae_sig n aes))
+  =
+  as_fun (ae0_composition n aes (KEY.key1_module n))
 
-#set-options "--z3rlimit 350 --max_fuel 3 --max_ifuel 4"
-let id_ae_module (n:u32) (km:module_t (key_sig n)) : module_t (sig_id_ae n) =
-  DM.create #_ #(sig_id_ae n).ops
-    (function ID_SET -> get_oracle km SET
-            | ID_CSET -> get_oracle km CSET)
+let ae_game1 n (aes:ae_scheme n)
+  : functor_t (sig_unit) (sig_prod (key_write_sig n) (ae_sig n aes))
+  =
+  as_fun (ae1_composition n aes (KEY.key1_module n))
 
-let id_ae_functor n
-  : functor_t (key_sig n) (sig_id_ae n)
-  = fun (k:module_t (key_sig n)) -> id_ae_module n k
+let ae_adversary n aes = atk (sig_unit) (sig_prod (key_write_sig n) (ae_sig n aes))
 
-//let ae_game0 n (aes:ae_scheme n) (km:module_t (key_sig n)) =
-//  functor_prod
-//    (key_sig n) (sig_id_gen n)
-//    (key_sig n) (sig_ae0 n aes)
-//    (id_ae_functor n)
-//    (ae0_functor n aes)
+assume val ae_eps: n:u32 -> aes:ae_scheme n -> eps (sig_unit) (sig_prod (key_write_sig n) (ae_sig n aes))
 
-let ae_game1 n (aes:ae_scheme n) (km:module_t (key_sig n)) =
-  functor_prod
-    (key_sig n) (sig_id_ae n)
-    (key_sig n) (sig_ae1 n aes)
-    (id_ae_functor n)
-    (ae1_functor n aes)
+let ae_functor_rel n aes : per (functor_t (sig_unit) (sig_prod (key_write_sig n) (ae_sig n aes))) =
+  fun funct_a funct_b -> True
+
+/// Questions:
+/// - What would a relation on a functor look like?
+/// - How to instantiate a hypothesis?
+let ae_assumption n aes = eq (ae_functor_rel n aes) (ae_eps n aes) (ae_game0 n aes) (ae_game1 n aes)
