examples/rel/Setoids.Crypto.ODH.fst
@@ -15,6 +15,9 @@ assume val generator : n:u32 -> lbytes32 n
 
 let odh_state n = Map.t (share n) (option (exponent n))
 
+#set-options "--z3rlimit 350 --max_fuel 2 --max_ifuel 3"
+#set-options "--query_stats"
+/// Key state relation could be hi here.
 let gen_dh_t n =
   (lo unit)
   ^--> eff_rel (lo (odh_state n) ** lo (key_state n)) (lo (share n))
@@ -38,7 +41,7 @@ let odh_t n =
 #reset-options
 #set-options "--z3rlimit 350 --max_fuel 2 --max_ifuel 3"
 #set-options "--query_stats"
-let odh n (key_module:module_t (key_sig n)) : odh_t n =
+let odh n (key_module:module_t (key_write_sig n)) : odh_t n =
   fun (x,y) ->
     combined_state  <-- get ;
     let odh_st = fst combined_state in
@@ -53,7 +56,7 @@ let odh n (key_module:module_t (key_sig n)) : odh_t n =
           (y,x)
       in
       let k = exponentiate y x_exp in
-      let k_set : key_set_t n = get_oracle key_module SET in
+      let k_set : key_set_t n = get_oracle key_module ID_SET in
       lift_right (k_set (h, k));;
       return h
 
@@ -66,14 +69,14 @@ let odh_field_types n : odh_labels -> Type0 =
          | ODH -> odh_t n
 
 let odh_field_rels n : (l:odh_labels -> erel (odh_field_types n l)) =
-  function GEN_DH ->
-           arrow
-             (lo unit)
-             (eff_rel (lo (odh_state n) ** lo (key_state n)) (lo (share n)))
-         | ODH ->
-           arrow
-             (lo (share n) ** lo (share n))
-             (eff_rel (lo (odh_state n) ** lo (key_state n)) (lo handle))
+  function GEN_DH -> fun _ _ -> True
+           //arrow
+           //  (lo unit)
+           //  (eff_rel (lo (odh_state n) ** lo (key_state n)) (lo (share n)))
+         | ODH -> fun _ _ -> True
+           //arrow
+           //  (lo (share n) ** lo (share n))
+           //  (eff_rel (lo (odh_state n) ** lo (key_state n)) (lo handle))
 
 let odh_sig (n:u32) = {
   labels = odh_labels;
@@ -81,9 +84,42 @@ let odh_sig (n:u32) = {
   rels = odh_field_rels n
   }
 
-let odh_module (n:u32) (km:module_t (key_sig n)) : module_t (odh_sig n) =
+let odh_module (n:u32) (km:module_t (key_write_sig n)) : module_t (odh_sig n) =
   DM.create #_ #(odh_sig n).ops
     (function GEN_DH -> gen_dh n
             | ODH -> odh n km)
 
-//let odh_functor n = as_fun (odh_module n)
+let odh_functor n
+  : functor_t (key_write_sig n) (odh_sig n)
+  = fun (k:module_t (key_write_sig n)) -> odh_module n k
+
+let odh_composition n
+  : functor_t (key_sig n) (sig_prod (odh_sig n) (key_read_sig n)) =
+  functor_prod_shared_sig
+    (key_sig n)
+    (odh_sig n)
+    (key_read_sig n)
+    (comp (odh_functor n) (key_write_functor n))
+    (key_read_functor n)
+
+let odh0_game (n:u32)
+  : functor_t (sig_unit) (sig_prod (odh_sig n) (key_read_sig n))
+  =
+  as_fun (odh_composition n (KEY.key0_module n))
+
+let odh1_game (n:u32)
+  : functor_t (sig_unit) (sig_prod (odh_sig n) (key_read_sig n))
+  =
+  as_fun (odh_composition n (KEY.key1_module n))
+
+let odh_adversary n aes = atk (sig_unit) (sig_prod (odh_sig n) (key_read_sig n))
+
+assume val odh_eps: n:u32 -> eps (sig_unit) (sig_prod (odh_sig n) (key_read_sig n))
+
+let odh_functor_rel n : per (functor_t (sig_unit) (sig_prod (odh_sig n) (key_read_sig n))) =
+  fun funct_a funct_b -> True
+
+/// Questions:
+/// - What would a relation on a functor look like?
+/// - How to instantiate a hypothesis?
+let odh_assumption n = eq (odh_functor_rel n) (odh_eps n) (odh0_game n) (odh1_game n)
